sf/Assignment08_04.v
@@ -13,7 +13,42 @@ Theorem no_whiles_terminate: forall c st
     (NOWHL: no_whiles c = true),
   exists st', c / st || st'.
 Proof.
-  exact FILL_IN_HERE.
+    intros.
+    generalize dependent st.
+    induction c; intros.
+    apply ex_intro with (x := st).
+    apply E_Skip.
+    apply ex_intro with (x := (update st i (aeval st a))).
+    apply E_Ass.
+    reflexivity.
+    inversion NOWHL.
+    apply andb_true_iff in H0.
+    inversion H0.
+    apply IHc1 with (st := st) in H.
+    inversion H.
+    apply IHc2 with (st := x) in H1.
+    inversion H1.
+    apply ex_intro with (x := x0).
+    apply E_Seq with (st' := x); assumption.
+    inversion NOWHL.
+    apply andb_true_iff in H0.
+    inversion H0.
+    apply IHc1 with (st := st) in H.
+    inversion H.
+    destruct (beval st b) eqn:b_dest.
+    apply ex_intro with (x := x).
+    apply E_IfTrue.
+    apply b_dest.
+    apply H2.
+    apply IHc2 with (st := st) in H1.
+    inversion H1.
+    apply ex_intro with (x := x0).
+    apply E_IfFalse.
+    apply b_dest.
+    apply H3.
+    destruct (beval st b) eqn:b_dest.
+    inversion NOWHL.
+    inversion NOWHL.
 Qed.
 
 (*-- Check --*)
