sf/Assignment08_07.v
@@ -9,7 +9,22 @@ Theorem IFB_false: forall b c1 c2,
     (IFB b THEN c1 ELSE c2 FI) 
     c2.
 Proof.
-  exact FILL_IN_HERE.
+    intros.
+    unfold cequiv.
+    intros.
+    unfold bequiv in H.
+    split.
+    intros.
+    inversion H0.
+    subst.
+    rewrite H in H6.
+    inversion H6.
+    subst.
+    apply H7.
+    intros.
+    apply E_IfFalse.
+    apply H.
+    apply H0.
 Qed.
 
 (*-- Check --*)
