sf/Assignment08_09.v
@@ -6,14 +6,47 @@ Require Export Assignment08_08.
 (** Prove the following theorem. _Hint_: You'll want to use
     [WHILE_true_nonterm] here. *)
 
+Lemma WHILE_true_nonterm : forall b c st st',
+     bequiv b BTrue ->
+     ~( (WHILE b DO c END) / st || st' ).
+Proof. 
+  (* WORKED IN CLASS *)
+  intros b c st st' Hb.
+  intros H.
+  remember (WHILE b DO c END) as cw.
+  ceval_cases (induction H) Case;
+    (* Most rules don't apply, and we can rule them out 
+       by inversion *)
+    inversion Heqcw; subst; clear Heqcw.
+  (* The two interesting cases are the ones for WHILE loops: *)
+  Case "E_WhileEnd". (* contradictory -- b is always true! *)
+unfold bequiv in Hb.
+    rewrite Hb in H. inversion H.
+  Case "E_WhileLoop". (* immediate from the IH *)
+    apply IHceval2. reflexivity.  Qed.
+
+
 Theorem WHILE_true: forall b c,
      bequiv b BTrue  ->
      cequiv 
        (WHILE b DO c END)
        (WHILE BTrue DO SKIP END).
 Proof. 
-  exact FILL_IN_HERE.
+    intros.
+    split.
+    intros.
+    apply ex_falso_quodlibet.
+    apply WHILE_true_nonterm in H0.
+    inversion H0.
+    apply H.
+    intros.
+    apply WHILE_true_nonterm in H0.
+    inversion H0.
+    unfold bequiv.
+    intros.
+    auto.
 Qed.
+   
 
 (*-- Check --*)
 Check WHILE_true: forall b c,
