sf/Assignment08_11.v
@@ -3,12 +3,58 @@ Require Export Assignment08_10.
 (* problem #11: 10 points *)
 
 (** **** Exercise: 2 stars (assign_aequiv)  *)
+Lemma update_same : forall st X n,
+    (update st X (st X)) n = st n.
+Proof.
+    intros.
+    unfold update.
+    destruct (eq_id_dec X n).
+    rewrite e.
+    auto.
+    auto.
+Qed.
+
+(*Lemma update_same_2 : forall st X,
+    update st X (st X) = st.
+Proof.
+    intros.*)
+    
+    
+
 Theorem assign_aequiv : forall X e,
   aequiv (AId X) e -> 
   cequiv SKIP (X ::= e).
 Proof.
-  exact FILL_IN_HERE.
+    intros.
+    split.
+    intros.
+    inversion H0.
+    subst.
+    unfold aequiv in H.
+    assert (st' = update st' X (aeval st' e)).
+        apply functional_extensionality.
+        intros.
+        rewrite <- H.
+        simpl.
+        symmetry.
+        rewrite update_same.
+        auto.
+    rewrite H1 at 2.
+    apply E_Ass.
+    auto.
+    intros.
+    assert (st = st').
+        apply functional_extensionality.
+        inversion H0;
+        subst.
+        rewrite <- H.
+        intros.
+        symmetry.
+        apply update_same.
+    rewrite H1.
+    apply E_Skip.
 Qed.
+       
 
 (*-- Check --*)
 Check assign_aequiv : forall X e,
