sf/Assignment08_12.v
@@ -7,7 +7,26 @@ Theorem CSeq_congruence : forall c1 c1' c2 c2',
   cequiv c1 c1' -> cequiv c2 c2' ->
   cequiv (c1;;c2) (c1';;c2').
 Proof. 
-  exact FILL_IN_HERE.
+    intros.
+    unfold cequiv in H.
+    unfold cequiv in H0.
+    split.
+    intros.
+    inversion H1.
+    subst.
+    apply E_Seq with st'0.
+    apply H.
+    apply H4.
+    apply H0.
+    apply H7.
+    intros.
+    inversion H1.
+    subst.
+    apply E_Seq with st'0.
+    apply H.
+    apply H4.
+    apply H0.
+    apply H7.
 Qed.
 
 (*-- Check --*)
