sf/Assignment08_13.v
@@ -7,7 +7,39 @@ Theorem CIf_congruence : forall b b' c1 c1' c2 c2',
   bequiv b b' -> cequiv c1 c1' -> cequiv c2 c2' ->
   cequiv (IFB b THEN c1 ELSE c2 FI) (IFB b' THEN c1' ELSE c2' FI).
 Proof.
-  exact FILL_IN_HERE.
+   intros.
+   unfold bequiv in H.
+   unfold cequiv in H0.
+   unfold cequiv in H1.
+   split.
+   intros.
+   inversion H2.
+   subst.
+   apply E_IfTrue.
+   rewrite <- H.
+   apply H8.
+   apply H0.
+   apply H9.
+   subst.
+   apply E_IfFalse.
+   rewrite <- H.
+   apply H8.
+   apply H1 in H9.
+   apply H9.
+   intros.
+   inversion H2.
+   subst.
+   apply E_IfTrue.
+   rewrite -> H.
+   apply H8.
+   apply H0.
+   apply H9.
+   subst.
+   apply E_IfFalse.
+   rewrite -> H.
+   apply H8.
+   apply H1 in H9.
+   apply H9.
 Qed.
 
 (*-- Check --*)
